src/Std/Data/DHashMap/Internal/RawLemmas.lean
@@ -3036,6 +3036,15 @@ theorem Equiv.inter_right {m₃ : Raw₀ α β} [EquivBEq α] [LawfulHashable α
   apply perm_filter_containsKey_of_perm equiv
   all_goals wf_trivial
 
+theorem Equiv.inter_congr {m₃ m₄ : Raw₀ α β} [EquivBEq α] [LawfulHashable α]
+    (h₁ : m₁.val.WF) (h₂ : m₂.val.WF) (h₃ : m₃.val.WF) (h₄ : m₄.val.WF) (equiv₁ : m₁.1.Equiv m₃.1) (equiv₂ :  m₂.1.Equiv m₄.1) :
+    (m₁.inter m₂).1.Equiv (m₃.inter m₄).1 := by
+  revert equiv₁ equiv₂
+  simp_to_model [Equiv, inter]
+  intro equiv₁ equiv₂
+  apply List.congr_filter_containsKey_of_perm
+  all_goals wf_trivial
+
 /- get? -/
 theorem get?_inter [LawfulBEq α] (h₁ : m₁.val.WF) (h₂ : m₂.val.WF) {k : α} :
     (m₁.inter m₂).get? k =
