src/Std/Data/Internal/List/Associative.lean
@@ -5503,6 +5503,16 @@ theorem perm_filter_containsKey_of_perm {l₁ l₂ l₃ : List ((a : α) × β a
     · simp only [List.perm_cons, ih]
     · simp [ih]
 
+theorem congr_filter_containsKey_of_perm {l₁ l₂ l₃ l₄ : List ((a : α) × β a)}
+    [BEq α] [EquivBEq α]
+    (h₁ : l₁.Perm l₃) (h₂ : l₂.Perm l₄)
+    (hd : DistinctKeys l₃) :
+    (l₁.filter (fun p => containsKey p.fst l₂)).Perm (l₃.filter (fun p => containsKey p.1 l₄)) := by
+  apply Perm.trans
+  · apply List.Perm.filter
+    · exact h₁
+  · apply perm_filter_containsKey_of_perm h₂ hd
+
 theorem List.getValue?_filter_containsKey {β : Type v} [BEq α] [EquivBEq α]
     {l₁ l₂ : List ((_ : α) × β)} {k : α}
     (dl₁ : DistinctKeys l₁) :
